specs/ecdsap256/Spec.ECC.fst
@@ -22,7 +22,6 @@ let pointAtInfinity #c : point_nat_prime #c  = (0, 0, 0)
 let isPointAtInfinity (p:point_nat) =
   let (_, _, z) = p in z = 0
 
-
 noextract
 let _point_double #curve (p:point_nat_prime #curve) : point_nat_prime #curve =
   let prime = getPrime curve in 
@@ -37,13 +36,13 @@ let _point_double #curve (p:point_nat_prime #curve) : point_nat_prime #curve =
   (x3, y3, z3)
 
 
-let _norm #curve (p:point_nat_prime #curve) : (point_nat_prime #curve) =
+ let _norm #curve (p:point_nat_prime #curve) : (point_nat_prime #curve) =
   let prime = getPrime curve in 
   let (x, y, z) = p in
   let z2 = z * z in
-  let z2i = modp_inv2_pow #curve z2 in
+  let z2i = modp_inv2 #curve z2 in
   let z3 = z * z * z in
-  let z3i = modp_inv2_pow #curve z3 in
+  let z3i = modp_inv2 #curve z3 in
   let x3 = (z2i * x) % prime in
   let y3 = (z3i * y) % prime in
   let z3 = if isPointAtInfinity p then 0 else 1 in
@@ -52,7 +51,7 @@ let _norm #curve (p:point_nat_prime #curve) : (point_nat_prime #curve) =
 
 let scalar_bytes (#c: curve) = lbytes (v (getScalarLenBytes c))
 
-let ith_bit (#c: curve) (k: scalar_bytes #c) (i:nat{i < getScalarLen c}) : (r: uint64 {v r == 0 \/ v r == 1}) =
+let ith_bit (#c: curve) (k: scalar_bytes #c) (i:nat{i < v (getScalarLen c)}) : (r: uint64 {v r == 0 \/ v r == 1}) =
   let q = (v (getScalarLenBytes c) - 1) - i / 8 in 
   let r = size (i % 8) in
   logand_mask (index k q >>. r) (u8 1) 1;
@@ -81,6 +80,7 @@ let pointEqual #curve (p: point_nat_prime #curve) (q: point_nat_prime #curve) =
   if (pAffineX = qAffineX && pAffineY = qAffineY) then 
     true
   else false
+
 
 
 noextract
@@ -140,17 +140,19 @@ let _ml_step1 #c r0 r1 =
   (r0, r1)
 
 
-val _ml_step: #c: curve -> k:scalar_bytes #c -> i:nat{i < getScalarLen c} 
+val _ml_step: #c: curve -> k: scalar_bytes #c -> i: nat{i < v (getScalarLen c)} 
   -> r: tuple2 (point_nat_prime #c) (point_nat_prime #c)
   -> tuple2 (point_nat_prime #c) (point_nat_prime #c)
 
 let _ml_step #c k i (p, q) =
-  let bit = (getPower c - 1) - i in
+  let bit = v (getScalarLen c) - 1 - i in
   let bit = ith_bit k bit in
   if uint_to_nat bit = 0 then
     _ml_step1 p q
   else
     _ml_step0 p q
+
+(* P + R == P + Q <==> R == Q --> P + P == P + Q <==> P == Q *)
 
 (* P + Q == Q + P *)
 assume val curve_commutativity_lemma: #c: curve -> p: point_nat_prime #c -> q: point_nat_prime #c -> Lemma 
@@ -168,6 +170,8 @@ assume val curve_multiplication_by_order: #c: curve -> i: int {(i + 1) % getOrde
 (* P + 0 == P *)
 assume val curve_point_at_infinity_property: #c: curve -> q: point_nat_prime #c -> Lemma (pointEqual (pointAdd pointAtInfinity q) q)
 
+assume val curve_associativity: #c: curve -> p: point_nat_prime #c -> q: point_nat_prime #c -> r: point_nat_prime #c -> Lemma 
+  (pointEqual (pointAdd (pointAdd p q) r) (pointAdd p (pointAdd q r)))
 
 val point_mult: #c: curve -> i: int -> p: point_nat_prime #c -> point_nat_prime #c
 
@@ -203,14 +207,102 @@ let point_mult_ext #c i p =
       lemma_mod_add_distr 1 (i - 1) (getOrder #c)
     end
 
+val lemma_test: #c: curve -> p: point_nat_prime #c -> pk: int -> Lemma (point_mult pk p == point_mult #c (pk % getOrder #c) p)
 
-assume val lemma_point_add : #c: curve -> p0: point_nat_prime #c -> pk: int -> qk: int -> i: int ->
-  Lemma (
+let lemma_test #c p pk = 
+  assert(point_mult pk p == repeat ((pk - 1) % getOrder #c) (fun x -> pointAdd #c p x) p);
+  assert(point_mult #c (pk % getOrder #c) p == repeat ((pk - 1) % getOrder #c % getOrder #c) (fun x -> pointAdd #c p x) p);
+  lemma_mod_twice (pk - 1) (getOrder #c)
+
+
+val point_mult_def: #c: curve -> i: int -> p: point_nat_prime #c -> Lemma 
+  (point_mult #c i p == repeat ((i - 1) % getOrder #c) (fun x -> pointAdd #c p x) p)
+
+let point_mult_def #c i p = ()
+
+#push-options "--z3rlimit 500"
+
+
+val lemma_test1: #c: curve -> p0: point_nat_prime #c  -> a: point_nat_prime #c -> b: point_nat_prime #c -> Lemma (
     let f = (fun x -> pointAdd #c p0 x) in 
-    let p = pointAdd (point_mult pk p0) (point_mult qk p0) in 
-    let p_i = pointAdd (point_mult (pk - i) p0) (point_mult (qk + i) p0) in 
-    pointEqual p p_i)
+    pointEqual (pointAdd (f a) b) (pointAdd (f b) a))
 
+let lemma_test1 #c p0 a b = 
+  let f = (fun x -> pointAdd #c p0 x) in 
+  curve_commutativity_lemma (f b) a;
+  curve_commutativity_lemma (pointAdd a (pointAdd p0 b)) (pointAdd (pointAdd p0 b) a);
+  curve_commutativity_lemma p0 a; 
+  curve_compatibility_with_translation_lemma (pointAdd p0 a) (pointAdd a p0) b;
+  curve_associativity a p0 b
+  
+
+val lemma_point_add: #c: curve -> p0: point_nat_prime #c -> pk: nat -> qk: nat -> i: nat -> Lemma (
+  let f = (fun x -> pointAdd #c p0 x) in 
+  let p = pointAdd (point_mult pk p0) (point_mult qk p0) in 
+  let p_i = pointAdd (point_mult (pk - i) p0) (point_mult (qk + i) p0) in 
+  pointEqual p p_i)
+
+let rec lemma_point_add #curve p0 pk qk i = 
+   match i with 
+  |0 -> ()
+  | _ -> 
+    let o = getOrder #curve in  
+    let f = (fun x -> pointAdd #curve p0 x) in 
+    lemma_point_add #curve p0 pk qk (i - 1);
+    
+    let p = pointAdd (point_mult pk p0) (point_mult qk p0) in 
+  
+    let a = (point_mult (pk - i + 1) p0) in 
+    let b = (point_mult (qk + i - 1) p0) in 
+    let c = (point_mult (pk - i) p0) in 
+    let d = (point_mult (qk + i) p0) in 
+
+    let p_i1 = pointAdd (point_mult (pk - i + 1) p0) (point_mult (qk + i - 1) p0) in 
+    let p_i = pointAdd (point_mult (pk - i) p0) (point_mult (qk + i) p0) in  
+
+    point_mult_def (pk - i + 1) p0;
+    point_mult_def (pk - i) p0;
+    unfold_repeat o f p0 ((pk - i - 1) % o);
+
+    curve_point_at_infinity_property #curve p0;
+    curve_commutativity_lemma pointAtInfinity p0;
+
+    if ((pk - i - 1) % o + 1) < o then 
+      begin
+	small_mod (((pk - i - 1) % o + 1)) o;
+	lemma_mod_add_distr 1 (pk - i - 1) o;
+	assert(pointEqual a (f c))
+      end 
+    else begin
+      curve_multiplication_by_order #curve ((pk - i - 1) % o) p0;
+      lemma_mod_add_distr 1 (pk - i - 1) o;
+      eq_repeat0 f p0;
+      assert(pointEqual a (f c))
+    end;
+
+
+    point_mult_def (qk + i - 1) p0;
+    point_mult_def (qk + i) p0;
+    unfold_repeat o f p0 ((qk + i - 1 - 1) % o);
+
+    if ((qk + i - 1 - 1) % o + 1) < o then 
+      begin 
+	small_mod (((qk + i - 1 - 1) % o) + 1) o;
+	lemma_mod_add_distr 1 (qk + i - 2) o;
+	assert (pointEqual d (f b))
+      end
+    else begin 
+      curve_multiplication_by_order #curve ((qk + i - 1 - 1) % o) p0;
+      lemma_mod_add_distr 1 (qk + i - 1) o;
+      eq_repeat0 f p0;
+      assert (pointEqual d (f b))
+    end;
+
+    curve_compatibility_with_translation_lemma a (f c) b;
+    curve_compatibility_with_translation_lemma d (f b) c;
+    curve_commutativity_lemma #curve d c;
+
+    lemma_test1 p0 c b
 
 
 val lemmaApplPointDouble: #c: curve 
@@ -220,9 +312,38 @@ val lemmaApplPointDouble: #c: curve
   Lemma (pointEqual (pointAdd p p) (point_mult (2 * pk) p0))
 
 let lemmaApplPointDouble #c p0 pk p =  
+  let o = getOrder #c in 
+
   let pk_p = point_mult pk p0 in 
-  
-  lemma_point_add #c p0 pk pk (pk - 1);
+
+  lemma_point_add #c p0 (pk % o) (pk % o) ((pk - 1) % o);
+  lemma_test p0 pk;
+
+  calc (==) {
+    point_mult (pk % o - ((pk - 1) % o)) p0;
+    (==) {lemma_test p0 (pk % o - ((pk - 1) % o))}
+    point_mult ((pk % o - ((pk - 1) % o)) % o) p0;
+    (==) {lemma_mod_add_distr (- ((pk - 1) % o)) pk o}
+    point_mult ((pk - ((pk - 1) % o)) % o) p0;
+    (==) {lemma_mod_sub_distr pk (pk - 1) o}
+    point_mult ((pk - (pk - 1)) % o) p0;
+    (==) {lemma_test p0 (pk - (pk - 1))}
+    point_mult ((pk - (pk - 1))) p0;
+  };
+
+  calc (==) {
+    point_mult (pk % o + ((pk - 1) % o)) p0;
+    (==) {lemma_test p0 (pk % o + ((pk - 1) % o))}
+    point_mult ((pk % o + ((pk - 1) % o)) % o) p0;
+    (==) {lemma_mod_add_distr ((pk - 1) % o) pk o}
+    point_mult ((pk + ((pk - 1) % o)) % o) p0;
+    (==) {lemma_mod_add_distr pk (pk - 1) o}
+    point_mult ((pk + pk - 1) % o) p0;
+    (==) {lemma_test p0 (pk + pk - 1)}
+    point_mult ((pk + pk - 1)) p0;
+    
+  };
+    
   point_mult_1 p0;
   point_mult_ext (2 * pk - 1) p0;
 
@@ -239,7 +360,8 @@ val lemmaApplPointAdd: #c: curve -> p0: point_nat_prime #c
 let lemmaApplPointAdd #c p0 pk p qk q = 
   let pk_p = point_mult pk p0 in 
   let qk_p = point_mult qk p0 in 
-  
+
+  (* to change *)
   lemma_point_add #c p0 qk pk (qk - 1);
   point_mult_1 p0;
   
