specs/ecdsap256/Spec.ECDSA.fst
@@ -1,4 +1,3 @@
-
 module Spec.ECDSA
 
 open FStar.Mul
@@ -20,7 +19,7 @@ open FStar.Math.Lib
 
 #set-options "--z3rlimit 200"
 
-val ith_bit_felem: #c: curve -> k:lbytes (getCoordinateLen c) -> i:nat{i < getPower c}
+val ith_bit_felem: #c: curve -> k: scalar_bytes #c -> i:nat{i < v (getScalarLen c)}
   -> t:uint64 {(v t == 0 \/ v t == 1) /\ v t == nat_from_intseq_le k / pow2 i % 2}
 
 let ith_bit_felem #c k i =
@@ -40,11 +39,12 @@ let ith_bit_felem #c k i =
   res
 
 
-let ( *% ) (#c: curve) a b = (a * b) % (getOrder #c)
+let ( *% ) (#c: curve) a b = (a * b) % getOrder #c
 
-let fmul (#c: curve) (a: elem (getPrime c)) (b: elem (getPrime c)) : elem (getPrime c) = (a * b) % (getPrime c)
+let fmul (#c: curve) (a: elem (getOrder #c)) (b: elem (getOrder #c)) : elem (getOrder #c) = a * b % getOrder #c
 
-val _exp_step0: #c: curve -> p: nat_prime #c -> q: nat_prime #c -> tuple2 (nat_prime #c) (nat_prime #c)
+
+val _exp_step0: #c: curve -> p: elem (getOrder #c) -> q: elem (getOrder #c) -> tuple2 (elem (getOrder #c)) (elem (getOrder #c))
 
 let _exp_step0 #c r0 r1 =
   let r1 = fmul #c r0 r1 in
@@ -52,7 +52,7 @@ let _exp_step0 #c r0 r1 =
   r0, r1
 
 
-val _exp_step1: #c: curve -> p:nat_prime #c -> q:nat_prime #c -> tuple2 (nat_prime #c) (nat_prime #c)
+val _exp_step1: #c: curve -> p: elem (getOrder #c) -> q: elem (getOrder #c) -> tuple2 (elem (getOrder #c)) (elem (getOrder #c))
 
 let _exp_step1 #c r0 r1 =
   let r0 = fmul #c r0 r1 in
@@ -62,54 +62,53 @@ let _exp_step1 #c r0 r1 =
 
 let swap p q = q, p
 
-val conditional_swap: #c: curve -> i:uint64 -> p: nat_prime #c -> q: nat_prime #c -> tuple2 (nat_prime #c) (nat_prime #c)
+
+val conditional_swap: #c: curve -> i:uint64 -> p: nat -> q: nat -> tuple2 nat nat
 
 let conditional_swap i p q =
   if v i = 0 then (p, q) else (q, p)
 
 
-val lemma_swaped_steps: #c: curve -> p: nat_prime #c -> q: nat_prime #c ->
-  Lemma (
-    let afterSwapP, afterSwapQ = swap p q in
-    let p1, q1 = _exp_step0 afterSwapP afterSwapQ in
-    let p2, q2 = swap p1 q1 in
-    let r0, r1 = _exp_step1 p q in
-    p2 == r0 /\ q2 == r1)
+val lemma_swaped_steps: #c: curve -> p: elem (getOrder #c) -> q: elem (getOrder #c) -> Lemma (
+  let afterSwapP, afterSwapQ = swap p q in
+  let p1, q1 = _exp_step0 afterSwapP afterSwapQ in
+  let p2, q2 = swap p1 q1 in
+  let r0, r1 = _exp_step1 p q in
+  p2 == r0 /\ q2 == r1)
 
 let lemma_swaped_steps p q = ()
 
 
 val _exp_step: #c: curve 
-  -> k:lseq uint8 (getCoordinateLen c) 
-  -> i:nat{i < getPower c} 
-  -> before:tuple2 (nat_prime #c) (nat_prime #c)
-  -> tuple2 (nat_prime #c) (nat_prime #c)
+  -> k: scalar_bytes #c
+  -> i: nat{i < v (getScalarLen c)} 
+  -> before: tuple2 (elem (getOrder #c)) (elem (getOrder #c))
+  -> tuple2 (elem (getOrder #c)) (elem (getOrder #c))
 
 let _exp_step #c k i (p, q) =
-  let bit = (getPower c - 1) - i in
-  let bit = ith_bit_felem k bit in
+  let bit0 = v (getScalarLen c) - 1 - i in
+  let bit = ith_bit_felem #c k bit0 in
   let open Lib.RawIntTypes in
-  if uint_to_nat bit = 0 then _exp_step0 p q else _exp_step1 p q
+  if uint_to_nat bit = 0 then _exp_step0 #c p q else _exp_step1 #c p q
 
 
 val _exponent_spec: #c: curve 
-  -> k:lseq uint8 (getCoordinateLen c) 
-  -> tuple2 (nat_prime #c) (nat_prime #c) 
-  -> tuple2 (nat_prime #c) (nat_prime #c)
+  -> k: scalar_bytes #c
+  -> tuple2 (elem (getOrder #c)) (elem (getOrder #c))
+  -> tuple2 (elem (getOrder #c)) (elem (getOrder #c))
 
 let _exponent_spec #c k (p, q) =
   let open Lib.LoopCombinators in
-  Lib.LoopCombinators.repeati (getPower c) (_exp_step k) (p, q)
+  Lib.LoopCombinators.repeati (v (getScalarLen c)) (_exp_step k) (p, q)
 
 
 val lemma_even: #c: curve 
-  -> index:pos{index <= getPower c} 
-  -> k:lseq uint8 (getCoordinateLen c) {v (ith_bit_felem k (getPower c - index)) == 0} ->
+  -> index: pos {index <= v (getScalarLen c)} 
+  -> k: scalar_bytes #c {v (ith_bit_felem #c k (v (getScalarLen c) - index)) == 0} ->
   Lemma (
     let number = nat_from_bytes_le k in
-    let newIndex = (getPower c) - index in
-    2 * arithmetic_shift_right number (newIndex + 1) ==
-    arithmetic_shift_right number newIndex)
+    let newIndex = v (getScalarLen c) - index in
+    2 * arithmetic_shift_right number (newIndex + 1) == arithmetic_shift_right number newIndex)
 
 let lemma_even #c index k =
   let number = nat_from_bytes_le k in
@@ -119,7 +118,8 @@ let lemma_even #c index k =
   FStar.Math.Lemmas.division_multiplication_lemma number (pow2 n) 2
 
 
-val lemma_odd: #c: curve -> index:pos{index <= getPower c} -> k:lseq uint8 (getCoordinateLen c) {uint_v (ith_bit_felem k (getPower c - index)) == 1} ->
+val lemma_odd: #c: curve -> index:pos{index <= getPower c} 
+  -> k:lseq uint8 (getCoordinateLen c) {uint_v (ith_bit_felem #c k (getPower c - index)) == 1} ->
   Lemma(
     let number = nat_from_intseq_le k in 
     let n = getPower c - index  in
@@ -145,7 +145,7 @@ val lemma_exponen_spec: #c: curve -> k:lseq uint8 (getCoordinateLen c)
     let start0, start1 = start in
     let number = nat_from_bytes_le k in
     let newIndex = getPower c - index in
-    let f0, f1 = Lib.LoopCombinators.repeati index (_exp_step k) start in
+    let f0, f1 = Lib.LoopCombinators.repeati index (_exp_step #c k) start in
     f0 == pow start1 (arithmetic_shift_right number newIndex) % getOrder #c /\
     f1 == pow start1 (arithmetic_shift_right number newIndex + 1) % getOrder #c
   )
@@ -158,7 +158,7 @@ val lemma_exponen_spec_0: #c: curve -> k:lseq uint8 (getCoordinateLen c)
     let start0, start1 = start in
     let number = nat_from_bytes_le k in
     let newIndex = getPower c in
-    let f0, f1 = Lib.LoopCombinators.repeati 0 (_exp_step k) start in
+    let f0, f1 = Lib.LoopCombinators.repeati 0 (_exp_step #c k) start in
     f0 == pow start1 (arithmetic_shift_right number newIndex) % getOrder #c /\
     f1 == pow start1 (arithmetic_shift_right number newIndex + 1) % getOrder #c
   )
@@ -169,7 +169,7 @@ let lemma_exponen_spec_0 #c k start =
   assert (arithmetic_shift_right number (getPower c) == number / pow2 (getPower c));
   FStar.Math.Lemmas.lemma_div_lt_nat number (getPower c) (getPower c);
   assert (arithmetic_shift_right number (getPower c) == 0);
-  Lib.LoopCombinators.eq_repeati0 (getPower c) (_exp_step k) start;
+  Lib.LoopCombinators.eq_repeati0 (getPower c) (_exp_step #c k) start;
   admit()
 
 #pop-options
@@ -178,7 +178,7 @@ let rec lemma_exponen_spec #c k start index =
   admit();
   let prime_order = getOrder #c in 
   let power = getPower c in 
-  let f = _exp_step k in
+  let f = _exp_step #c k in
   let st0, st1 = start in
   let number = nat_from_bytes_le k in
   let newIndex = getPower c - index in
@@ -189,7 +189,7 @@ let rec lemma_exponen_spec #c k start index =
     begin
     unfold_repeati (getPower c) f start (index - 1);
     lemma_exponen_spec k start (index - 1);
-    let bitMask = uint_v (ith_bit_felem k ((getPower c) - index)) in
+    let bitMask = uint_v (ith_bit_felem #c k ((getPower c) - index)) in
     match bitMask with
       | 0 ->
         let a0 = pow st1 (arithmetic_shift_right number (power - index + 1)) in
@@ -204,7 +204,7 @@ let rec lemma_exponen_spec #c k start index =
           (pow st1 (arithmetic_shift_right number (power - index + 1) + arithmetic_shift_right number (power - index + 1))) % prime_order;
           == {}
           (pow st1 (2 * arithmetic_shift_right number (power - index + 1))) % prime_order;
-          == {lemma_even index k}
+          == {lemma_even #c index k}
           pow st1 (arithmetic_shift_right number newIndex) % prime_order;
         };
         calc (==) {
@@ -217,7 +217,7 @@ let rec lemma_exponen_spec #c k start index =
           (pow st1 (arithmetic_shift_right number (power - index + 1) + arithmetic_shift_right number (power - index + 1) + 1)) % prime_order;
           == {}
           (pow st1 (2 * arithmetic_shift_right number (power - index + 1) + 1)) % prime_order;
-          == {lemma_even index k}
+          == {lemma_even #c index k}
           (pow st1 (arithmetic_shift_right number (power - index) + 1)) % prime_order;
         }
       | 1 ->
@@ -312,15 +312,15 @@ let prime_order_seq (#c: curve) : s:lseq uint8 (getCoordinateLen c)
   of_list (prime_order_list #c)
 
 
-val exponent_spec: #c: curve -> a:nat_prime #c -> r:nat_prime #c{r = pow a (getOrder #c - 2) % getOrder #c}
+val exponent_spec: #c: curve -> a: elem (getOrder #c) -> r: elem (getOrder #c) {r = pow a (getOrder #c - 2) % getOrder #c}
 
 let exponent_spec #c a =
-  let a0, _ = _exponent_spec prime_order_inverse_seq (1, a) in
-  lemma_exponen_spec prime_order_inverse_seq (1, a) (getPower c) ;
+  let a0, _ = _exponent_spec (prime_order_inverse_seq #c) (1, a) in
+  lemma_exponen_spec (prime_order_inverse_seq #c) (1, a) (getPower c) ;
   a0
 
 
-
+(* The last check should be done only if the group is not prime *)
 val verifyQValidCurvePointSpec: #c: curve 
   -> publicKey:tuple3 nat nat nat{~(isPointAtInfinity publicKey)} -> bool
 
@@ -334,6 +334,7 @@ let verifyQValidCurvePointSpec #c publicKey =
   isPointAtInfinity (scalar_multiplication #c (prime_order_seq #c) publicKey)
 
 
+(* Check that {\displaystyle Q_{A}}Q_{A} is not equal to the identity element O, and its coordinates are otherwise valid *)
 val checkCoordinates: #c: curve ->  r: nat -> s: nat -> bool
 
 let checkCoordinates #c r s =
@@ -341,6 +342,7 @@ let checkCoordinates #c r s =
   if r > 0 && r < prime && s > 0 && s < prime
   then true
   else false
+
 
 open Spec.Hash.Definitions
 
@@ -353,8 +355,7 @@ let invert_state_s (a: hash_alg_ecdsa): Lemma
   (requires True)
   (ensures (inversion hash_alg_ecdsa))
   [ SMTPat (hash_alg_ecdsa) ]
-=
-  allow_inversion (hash_alg_ecdsa)
+  = allow_inversion (hash_alg_ecdsa)
 
 
 val min_input_length: #c: curve -> hash_alg_ecdsa -> Tot int
@@ -364,24 +365,19 @@ let min_input_length #c a =
     |NoHash -> getCoordinateLen c
     |Hash a -> 0
 
+
 (* Calculate {\displaystyle e={\textrm {HASH}}(m)}e={\textrm {HASH}}(m). (Here HASH is a cryptographic hash function, such as SHA-2, with the output converted to an integer.)
 Let {\displaystyle z}z be the {\displaystyle L_{n}}L_{n} leftmost bits of {\displaystyle e}e, where {\displaystyle L_{n}}L_{n} is the bit length of the group order {\displaystyle n}n. (Note that {\displaystyle z}z can be greater than {\displaystyle n}n but not longer.[1]) *)
 
-
-(* Not decided yet *)
 val hashSpec:
   c: curve 
   -> a: hash_alg_ecdsa 
   -> mLen: size_nat{mLen >= min_input_length #c a}
   -> m: lseq uint8 mLen ->
-  Tot (Lib.ByteSequence.lbytes 
-    (
-      if NoHash? a 
-	then getCoordinateLen c 
-      else if hash_length (match a with Hash a -> a) > getCoordinateLen c
-	then getCoordinateLen c 
-      else hash_length (match a with Hash a -> a) 
-))
+  Tot (Lib.ByteSequence.lbytes (
+    if NoHash? a then getCoordinateLen c 
+    else if hash_length (match a with Hash a -> a) > getCoordinateLen c
+    then getCoordinateLen c else hash_length (match a with Hash a -> a)))
 
 let hashSpec c a mLen m = 
   assert_norm (pow2 32 < pow2 61);
@@ -395,8 +391,6 @@ let hashSpec c a mLen m =
       sub hashed 0 (getCoordinateLen c)
     else
       hashed
-
-open Lib.ByteSequence 
 
 
 val ecdsa_verification_agile:
@@ -419,14 +413,14 @@ let ecdsa_verification_agile c alg publicKey r s mLen m =
     if not ((checkCoordinates #c) r s) then false
     else
       begin
-
       let hashM = hashSpec c alg mLen m in
       let hashNat = nat_from_bytes_be hashM % order in 
 
       let u1 = nat_to_bytes_be (getCoordinateLen c) (pow s (order - 2) * hashNat % order) in
       let u2 = nat_to_bytes_be (getCoordinateLen c) (pow s (order - 2) * r % order) in 
 
-      let pointAtInfinity = (0, 0, 0) in
+      point_mult_0 (basePoint #c) 0;
+      point_mult_0 #c publicJacobian 0;
       let u1D, _ = montgomery_ladder_spec_left #c u1 (pointAtInfinity, basePoint #c) in
       let u2D, _ = montgomery_ladder_spec_left #c u2 (pointAtInfinity, publicJacobian) in
 
@@ -444,22 +438,23 @@ val ecdsa_signature_agile:
   -> alg: hash_alg_ecdsa
   -> mLen:size_nat{mLen >= min_input_length #c alg} 
   -> m:lseq uint8 mLen
-  -> privateKey:lseq uint8 32
-  -> k:lseq uint8 32
+  -> privateKey: scalar_bytes #c
+  -> k: scalar_bytes #c
   -> tuple3 nat nat uint64
 
 let ecdsa_signature_agile c alg mLen m privateKey k =
   assert_norm (pow2 32 < pow2 61);
   assert_norm (pow2 32 < pow2 125);
-  let order = getOrder #c in 
-  let r, _ = montgomery_ladder_spec_left #c k ((0,0,0), (basePoint #c)) in
+  let prime_order = getOrder #c in 
+    point_mult_0 (basePoint #c) 0;
+  let r, _ = montgomery_ladder_spec_left #c k (pointAtInfinity, (basePoint #c)) in
   let (xN, _, _) = _norm #c r in
   let hashM = hashSpec c alg mLen m in 
-  let z = nat_from_bytes_be hashM % order in
+  let z = nat_from_bytes_be hashM % prime_order in
   let kFelem = nat_from_bytes_be k in
   let privateKeyFelem = nat_from_bytes_be privateKey in
-  let resultR = xN % order in
-  let resultS = (z + resultR * privateKeyFelem) * pow kFelem (order - 2) % order in
+  let resultR = xN % prime_order in
+  let resultS = (z + resultR * privateKeyFelem) * pow kFelem (prime_order - 2) % prime_order in
     if resultR = 0 || resultS = 0 then
       resultR, resultS, u64 (pow2 64 - 1)
     else
