code/ecdsa/Hacl.Impl.EC.MontgomeryLadder.fst
@@ -1,0 +1,320 @@
+module Hacl.Impl.EC.MontgomeryLadder
+
+open FStar.HyperStack.All
+open FStar.HyperStack
+module ST = FStar.HyperStack.ST
+
+open Lib.IntTypes
+open Lib.Buffer
+
+open Hacl.Spec.EC.Definition
+open Spec.ECC
+open Spec.ECC.Curves
+
+open Hacl.Impl.EC.PointAdd
+open Hacl.Impl.P.PointAdd.Aux
+open Hacl.Impl.EC.PointDouble
+
+open Lib.Loops
+
+open Hacl.Lemmas.P256
+
+open FStar.Mul
+open Hacl.Spec.MontgomeryMultiplication
+
+
+#set-options " --z3rlimit 200"
+
+val scalar_bit: #c: curve 
+  -> #buf_type: buftype 
+  -> s:lbuffer_t buf_type uint8 (getScalarLenBytes c) 
+  -> n:size_t{v n < v (getScalarLen c)}
+  -> Stack uint64
+    (requires fun h0 -> live h0 s)
+    (ensures  fun h0 r h1 -> h0 == h1 /\ r == ith_bit #c (as_seq h0 s) (v n) /\ v r <= 1)
+
+let scalar_bit #c #buf_type s n =
+  let h0 = ST.get () in
+  assert_norm (1 = pow2 1 - 1);
+  assert (v (mod_mask #U8 #SEC 1ul) == v (u8 1)); 
+  to_u64 ((s.(getScalarLenBytes c -. 1ul -. n /. 8ul) >>. (n %. 8ul)) &. u8 1)
+
+
+val swap: #c: curve ->  p: point_seq c -> q: point_seq c -> 
+  Tot (r: tuple2 (point_seq c) (point_seq c) {let pNew, qNew = r in pNew == q /\ qNew == p})
+
+let swap p q = (q, p)
+
+
+val conditional_swap: #c: curve -> i: uint64 -> p: point_seq c -> q: point_seq c -> 
+  Tot (r: tuple2 (point_seq c) (point_seq c) {
+    let pNew, qNew = r in 
+    if uint_v i = 0 then pNew == p /\ qNew == q
+    else let p1, q1 = swap p q in p1 == pNew /\ q1 == qNew})
+
+let conditional_swap i p q = 
+  if uint_v i = 0 then (p, q) else (q, p)
+
+
+val lemma_point_eval_swapped: c: curve -> h0: mem -> h1: mem -> p: point c -> q: point c ->
+  Lemma (requires (point_eval c h0 p /\ as_seq h0 p == as_seq h1 q))
+  (ensures (point_eval c h1 q))
+
+let lemma_point_eval_swapped c h0 h1 p q = 
+  assert(
+  as_nat c h0 (gsub p (size 2 *! getCoordinateLenU64 c) (getCoordinateLenU64 c)) == 
+  as_nat c h1 (gsub q (size 2 *! getCoordinateLenU64 c) (getCoordinateLenU64 c)))
+
+
+val lemma_PointEqualR: #c: curve -> p: point_nat_prime #c -> q: point_nat_prime #c -> Lemma
+  ((~ (pointEqual p q)) <==> ~ (pointEqual q p))
+
+let lemma_PointEqualR #c p q = ()
+
+val lemma_point_as_nat: #c: curve -> h: mem -> h1: mem 
+  -> p: point c {point_eval c h p} 
+  -> q: point c -> Lemma
+  (as_seq h p == as_seq h1 q ==> point_as_nat c h p == point_as_nat c h1 q)
+
+let lemma_point_as_nat #c h h1 p q = 
+  let len = getCoordinateLenU64 c in 
+  
+  let pX = gsub p (size 0) len in 
+  let pY = gsub p len len in 
+  let pZ = gsub p (size 2 *! len) len in 
+  
+  let qX = gsub q (size 0) len in 
+  let qY = gsub q len len in 
+  let qZ = gsub q (size 2 *! len) len in 
+
+  lemma_equal_lseq_equal_nat (as_seq h pX) (as_seq h1 qX);
+  lemma_equal_lseq_equal_nat (as_seq h pY) (as_seq h1 qY);
+  lemma_equal_lseq_equal_nat (as_seq h pZ) (as_seq h1 qZ)
+
+
+[@ CInline]
+val cswap: #c: curve -> bit:uint64{v bit <= 1} -> p:point c -> q:point c-> 
+  Stack unit
+  (requires fun h -> live h p /\ live h q /\ eq_or_disjoint p q /\ point_eval c h p /\ point_eval c h q /\
+    ~ (pointEqual #c
+      (let pX, pY, pZ = point_as_nat c h p in fromDomain #c pX, fromDomain #c pY, fromDomain #c pZ) 
+      (let qX, qY, qZ = point_as_nat c h q in fromDomain #c qX, fromDomain #c qY, fromDomain #c qZ)))
+  (ensures  fun h0 _ h1 -> modifies (loc p |+| loc q) h0 h1 /\
+    point_eval c h1 p /\ point_eval c h1 q /\ (
+    v bit == 0 ==> point_as_nat c h1 p == point_as_nat c h0 p /\ point_as_nat c h1 q == point_as_nat c h0 q) /\ (
+    v bit == 1 ==> point_as_nat c h1 p == point_as_nat c h0 q /\ point_as_nat c h1 q == point_as_nat c h0 p) /\
+    ~ (pointEqual #c (fromDomainPoint #c #DH (point_as_nat c h1 p)) (fromDomainPoint #c #DH (point_as_nat c h1 q))))
+
+let cswap #c bit p1 p2 =
+  let open Lib.Sequence in 
+  let h0 = ST.get () in
+  let mask = u64 0 -. bit in
+  
+  let len = getCoordinateLenU64 c *! size 3 in 
+
+  [@ inline_let]
+  let inv h1 (i:nat{i <= uint_v (getCoordinateLenU64 c) * 3}) =
+    (forall (k:nat{k < i}).
+      if v bit = 1
+      then (as_seq h1 p1).[k] == (as_seq h0 p2).[k] /\ (as_seq h1 p2).[k] == (as_seq h0 p1).[k]
+      else (as_seq h1 p1).[k] == (as_seq h0 p1).[k] /\ (as_seq h1 p2).[k] == (as_seq h0 p2).[k]) /\
+    (forall (k:nat{i <= k /\ k < uint_v (getCoordinateLenU64 c) * 3}).
+      (as_seq h1 p1).[k] == (as_seq h0 p1).[k] /\ (as_seq h1 p2).[k] == (as_seq h0 p2).[k]) /\
+    modifies (loc p1 |+| loc p2) h0 h1 in
+ 
+  Lib.Loops.for 0ul len inv
+    (fun i ->
+      let dummy = mask &. (p1.(i) ^. p2.(i)) in
+      p1.(i) <- p1.(i) ^. dummy;
+      p2.(i) <- p2.(i) ^. dummy;
+      lemma_cswap2_step bit ((as_seq h0 p1).[v i]) ((as_seq h0 p2).[v i])
+    );
+  let h1 = ST.get () in
+  
+  Lib.Sequence.eq_intro (as_seq h1 p1) (if v bit = 1 then as_seq h0 p2 else as_seq h0 p1);
+  Lib.Sequence.eq_intro (as_seq h1 p2) (if v bit = 1 then as_seq h0 p1 else as_seq h0 p2);
+
+  if v bit = 1 then begin
+    lemma_point_eval_swapped c h0 h1 p1 p2; 
+    lemma_point_as_nat #c h0 h1 p1 p2;
+    lemma_point_as_nat #c h0 h1 p2 p1;
+    lemma_point_eval_swapped c h0 h1 p2 p1 
+    end
+  else begin
+    lemma_point_eval c h0 h1 p1;
+    lemma_point_as_nat #c h0 h1 p1 p1;
+    lemma_point_as_nat #c h0 h1 p2 p2;
+    lemma_point_eval c h0 h1 p2 end
+
+
+val pointAddAsAdd: #c: curve -> p: point_nat_prime #c -> q: point_nat_prime #c -> Lemma
+    (requires (~ (pointEqual p q)))
+    (ensures (pointAdd p q == _point_add p q))
+
+let pointAddAsAdd #c p q = ()
+
+val pointAddAsDouble: #c: curve -> p: point_nat_prime #c -> q: point_nat_prime #c -> Lemma
+  (requires (True))
+  (ensures (pointAdd p p == _point_double p))
+
+let pointAddAsDouble #c p q = ()
+
+
+val point_add_as_spec: #c: curve -> p: point c -> q: point c -> result: point c 
+  -> tempBuffer: lbuffer uint64 (size 17 *! getCoordinateLenU64 c) -> 
+  Stack unit (requires fun h -> 
+    live h p /\ live h q /\ live h result /\ live h tempBuffer /\ 
+    eq_or_disjoint q result /\ disjoint p q /\ disjoint p tempBuffer /\ 
+    disjoint q tempBuffer /\ disjoint p result /\ disjoint result tempBuffer /\  
+    point_eval c h p /\ point_eval c h q /\ 
+    ~ (pointEqual #c (fromDomainPoint #c #DH (point_as_nat c h p)) (fromDomainPoint #c #DH (point_as_nat c h q))))
+  (ensures fun h0 _ h1 -> 
+    modifies (loc tempBuffer |+| loc result) h0 h1 /\ point_eval c h1 result /\ point_eval c h1 p /\ (
+    let pD = fromDomainPoint #c #DH (point_as_nat c h0 p) in 
+    let qD = fromDomainPoint #c #DH (point_as_nat c h0 q) in 
+    fromDomainPoint #c #DH (point_as_nat c h1 result) == pointAdd #c pD qD /\ 
+    point_as_nat c h0 p == point_as_nat c h1 p))
+
+
+let point_add_as_spec #c p q result tempBuffer = 
+    let h0 = ST.get() in 
+  point_add #c p q result tempBuffer;
+    let h1 = ST.get() in 
+  pointAddAsAdd #c 
+    (let pX, pY, pZ = point_as_nat c h0 p in fromDomain #c pX, fromDomain #c pY, fromDomain #c pZ)
+    (let qX, qY, qZ = point_as_nat c h0 q in fromDomain #c qX, fromDomain #c qY, fromDomain #c qZ);
+  lemma_coord_eval c h0 h1 p
+  
+
+val montgomery_ladder_step1: #c : curve -> p: point c -> q: point c 
+  -> tempBuffer: lbuffer uint64 (size 17 *! getCoordinateLenU64 c) -> Stack unit
+  (requires fun h ->  live h p /\ live h q /\ live h tempBuffer /\ 
+    LowStar.Monotonic.Buffer.all_disjoint [loc p; loc q; loc tempBuffer] /\
+    point_eval c h p /\ point_eval c h q /\
+    ~ (pointEqual #c (fromDomainPoint #c #DH (point_as_nat c h p)) (fromDomainPoint #c #DH (point_as_nat c h q))))
+  (ensures fun h0 _ h1 -> modifies (loc p |+| loc q |+| loc tempBuffer) h0 h1 /\ 
+    point_eval c h1 p /\ point_eval c h1 q /\ (
+    let ml1p, ml1q = _ml_step1 #c (fromDomainPoint #c #DH (point_as_nat c h0 p)) (fromDomainPoint #c #DH (point_as_nat c h0 q)) in 
+    ml1p == fromDomainPoint #c #DH (point_as_nat c h1 p) /\ ml1q == fromDomainPoint #c #DH (point_as_nat c h1 q) /\
+    ~ (pointEqual #c (fromDomainPoint #c #DH (point_as_nat c h1 p)) (fromDomainPoint #c #DH (point_as_nat c h1 q)))))
+
+
+let montgomery_ladder_step1 #c p q tempBuffer = 
+  let h0 = ST.get() in
+  point_add_as_spec p q q tempBuffer;
+    let h1 = ST.get() in 
+  point_double p p tempBuffer; 
+    let h2 = ST.get() in 
+  lemma_point_eval c h1 h2 q;
+  lemma_coord_eval c h1 h2 q;
+  pointAddAsDouble #c (fromDomainPoint #c #DH (point_as_nat c h0 p)) (fromDomainPoint #c #DH (point_as_nat c h0 p));
+  assume ( ~ (pointEqual #c (fromDomainPoint #c #DH (point_as_nat c h2 p)) (fromDomainPoint #c #DH (point_as_nat c h2 q))))
+
+
+val _montgomery_ladder_step: #c: curve -> #buf_type: buftype
+  -> p: point c -> q: point c 
+  -> tempBuffer: lbuffer uint64 (size 17 *! getCoordinateLenU64 c) 
+  -> bit: uint64 {v bit <= 1} ->
+  Stack unit
+  (requires fun h -> live h p /\ live h q /\ live h tempBuffer /\ point_eval c h p /\ point_eval c h q  /\
+    LowStar.Monotonic.Buffer.all_disjoint [loc p; loc q; loc tempBuffer] /\
+    ~ (pointEqual #c (fromDomainPoint #c #DH (point_as_nat c h p)) (fromDomainPoint #c #DH (point_as_nat c h q))))
+  (ensures fun h0 _ h1 -> modifies (loc p |+| loc q |+| loc tempBuffer) h0 h1 /\ 
+    point_eval c h1 p /\ point_eval c h1 q /\ (
+    let pM1, qM1 = _ml_step1 #c (fromDomainPoint #c #DH (point_as_nat c h0 p)) (fromDomainPoint #c #DH (point_as_nat c h0 q)) in
+    let pM0, qM0 = _ml_step0 #c (fromDomainPoint #c #DH (point_as_nat c h0 p)) (fromDomainPoint #c #DH (point_as_nat c h0 q)) in
+    
+    (~ (pointEqual #c (fromDomainPoint #c #DH (point_as_nat c h1 p)) (fromDomainPoint #c #DH (point_as_nat c h1 q))) /\ (
+    if v bit = 0 then 
+      fromDomainPoint #c #DH (point_as_nat c h1 p) == pM1 /\
+      fromDomainPoint #c #DH (point_as_nat c h1 q) == qM1 
+    else 
+      fromDomainPoint #c #DH (point_as_nat c h1 p) == pM0 /\
+      fromDomainPoint #c #DH (point_as_nat c h1 q) == qM0))))
+
+
+let _montgomery_ladder_step #c #buf_type r0 r1 tempBuffer bit = 
+  cswap bit r0 r1; 
+  montgomery_ladder_step1 r0 r1 tempBuffer;
+  cswap bit r0 r1
+
+
+val montgomery_ladder_step: #c: curve -> #buf_type: buftype
+  -> p: point c -> q: point c 
+  -> tempBuffer: lbuffer uint64 (size 17 *! getCoordinateLenU64 c) 
+  -> scalar: lbuffer_t buf_type uint8 (getScalarLenBytes c) 
+  -> i:size_t {v i < v (getScalarLen c)} -> 
+  Stack unit
+  (requires fun h -> live h p /\ live h q /\ live h tempBuffer /\ live h scalar /\
+    LowStar.Monotonic.Buffer.all_disjoint [loc p; loc q; loc tempBuffer; loc scalar] /\
+    point_eval c h p /\ point_eval c h q /\
+    ~ (pointEqual #c (fromDomainPoint #c #DH (point_as_nat c h p)) (fromDomainPoint #c #DH (point_as_nat c h q))))
+  (ensures fun h0 _ h1 -> modifies (loc p |+| loc q |+| loc tempBuffer) h0 h1 /\ 
+    point_eval c h1 p /\ point_eval c h1 q /\ (
+    let pM, qM = _ml_step #c (as_seq h0 scalar) (v i) (
+      fromDomainPoint #c #DH (point_as_nat c h0 p), fromDomainPoint #c #DH (point_as_nat c h0 q)) in    
+    fromDomainPoint #c #DH (point_as_nat c h1 p) == pM /\ fromDomainPoint #c #DH (point_as_nat c h1 q) == qM))
+
+let montgomery_ladder_step #c #buf_type r0 r1 tempBuffer scalar i = 
+  let bit0 = getScalarLen c -! 1ul -! i in 
+  let bit = scalar_bit scalar bit0 in 
+  _montgomery_ladder_step #c #buf_type r0 r1 tempBuffer bit
+
+
+val montgomery_ladder: #c: curve -> #buf_type: buftype -> p: point c -> q: point c ->
+  scalar: lbuffer_t buf_type uint8 (getScalarLen c) -> 
+  tempBuffer: lbuffer uint64 (size 17 *! getCoordinateLenU64 c)  -> 
+  Stack unit
+  (requires fun h -> live h p /\ live h q /\ live h scalar /\  live h tempBuffer /\
+    LowStar.Monotonic.Buffer.all_disjoint [loc p; loc q; loc tempBuffer; loc scalar] /\
+    point_eval c h p /\ point_eval c h q /\
+    pointEqual #c (fromDomainPoint #c #DH (point_as_nat c h p) (point_mult #c 0 (fromDomainPoint #c #DH (point_as_nat c h q)) /\
+    ~ (pointEqual #c (fromDomainPoint #c #DH (point_as_nat c h p)) (fromDomainPoint #c #DH (point_as_nat c h q))))
+  (ensures fun h0 _ h1 -> modifies (loc p |+| loc q |+| loc tempBuffer) h0 h1 /\
+    point_eval c h1 p /\ point_eval c h1 q /\ (admit();
+    let p1 = fromDomainPoint #c #DH (point_as_nat c h1 p) in 
+    let q1 = fromDomainPoint #c #DH (point_as_nat c h1 q) in 
+    let rN, qN = montgomery_ladder_spec_left #c (as_seq h0 scalar) (
+    fromDomainPoint #c #DH (point_as_nat c h0 p),  
+    fromDomainPoint #c #DH (point_as_nat c h0 q)) in 
+    rN == p1 /\ qN == q1))
+
+ 
+
+let montgomery_ladder #c #a p q scalar tempBuffer =  
+  let h0 = ST.get() in 
+
+  [@inline_let]
+  let len = getCoordinateLenU64 c in 
+  let cycleLoop = getPowerU c in 
+
+  [@inline_let]
+  let spec_ml h0 = _ml_step #c (as_seq h0 scalar) in 
+
+  [@inline_let] 
+  let acc (h:mem) : GTot (tuple2 point_nat_prime point_nat_prime) = 
+  (fromDomainPoint #c #DH (point_prime_to_coordinates c (as_seq h p)),
+  fromDomainPoint #c #DH (point_prime_to_coordinates c (as_seq h q)))  in 
+  
+  Lib.LoopCombinators.eq_repeati0 (getPower c) (spec_ml h0) (acc h0);
+  [@inline_let]
+  let inv h (i: nat {i <= getPower c}) = 
+    as_nat c h (gsub p (size 0) len) < getPrime c /\ 
+    as_nat c h (gsub p len len) < getPrime c /\
+    as_nat c h (gsub p (size 2 *! len) len) < getPrime c /\
+	
+    as_nat c h (gsub q (size 0) len) < getPrime c /\  
+    as_nat c h (gsub q len len) < getPrime c /\
+    as_nat c h (gsub q (size 2 *! len) len) < getPrime c /\
+    modifies3 p q tempBuffer h0 h   /\
+    acc h == Lib.LoopCombinators.repeati i (spec_ml h0) (acc h0)
+
+    in 
+
+  for 0ul cycleLoop inv 
+    (fun i -> let h2 = ST.get() in
+      montgomery_ladder_step p q tempBuffer scalar i; 
+      Lib.LoopCombinators.unfold_repeati (getPower c) (spec_ml h0) (acc h0) (uint_v i)
+    );
+    admit()
+
